Implemented multiple renamings, used to prove beta reduction substitution lemma. All unproven lemmas are now basic facts about substitutions and renamings! But not sure what kind of preconditions they will require and where to start proving.

src/PlutusIR/Semantics/Static/normaliser/SN_STLC_named.v
@@ -82,7 +82,6 @@ Proof. move->. exact: step_beta. Qed.
 Lemma capmsRename x x' t sigma s :
   ((x', t)::sigma) [[rename x x' s]] = ((x, t)::sigma) [[s]].
 Proof. 
-  
 Admitted.
 
 Definition notKeyIn X (sigma : list (string * term)) : Prop :=
@@ -123,6 +122,44 @@ Lemma commute_subst s t sigma x :
 Proof.
 Admitted.
 
+(* Stepping does not change free vars*)
+Lemma step_preserves_fresh_sigma s t1 t2 x : step t1 t2 -> fresh2 [(x, t1)] s = fresh2 [(x, t2)] s.
+Proof.
+Admitted.
+
+Lemma step_preserves_fresh sigma t1 t2 : 
+  step t1 t2 -> fresh2 sigma t1 = fresh2 sigma t2.
+Proof.
+Admitted.
+
+(* TODO: Not true because of fresh, what conditions do we need? *)
+(* e.g. rename X Y (tmlam Y A (tmvar X)) = tmlam Y A (tmvar Y). 
+  that case shouldnt be possible. But Y is not in ftv (tmlam Y A (tmvar X))
+  should we consider all type variables, not only the free ones for ftv?
+
+*)
+Lemma ren_is_subst : forall X X' s,
+  rename X X' s = [X := tmvar X'] s.
+Proof.
+Abort.
+
+(* TODO: some conditions necessary like X'  not in sigma*)
+Lemma ren_sub_compose : forall sigma X X' s,
+  sigma [[rename X X' s]] = ((X, tmvar X')::sigma) [[s]].
+Proof.
+  (* This is not exactly true, since rename does not create fresh vars and stuff
+        But it is "kind of true" , lol.
+
+        So I guess we have to change capms to not unnecessarily rename?
+        I would rather not ;) Maybe we can strengthen IHh to include this case.
+        Or we change rename to do fresh?
+
+        But it should be true, the fact that x' is fresh is key. that will mean that
+        capms and rename should behave the same in the tylam case
+        SO: TODO: We have to change capms to not freshen if not necessary
+      *)
+      
+Admitted.
 
 (* Note: Study: After replacing a variable with something in sigma
   we can still do the same step as we previously could by red s t, hence: true
@@ -158,37 +195,13 @@ Proof.
   - rewrite capms_equation_2.
     rewrite capms_equation_2.
     simpl.
-    remember (fresh2 sigma s1) as x_s1.
-    remember (fresh2 sigma s2) as x_s2.
-    assert (H_xeq: x_s1 = x_s2). {
-      (* Problem: Fresh variables get out of sync.
-      or maybe not: the ftv in s1 and s2 are the same.
-      Stepping does not remove free vars, ftv s1 = ftv s2!
-      So fresh2 sigma s1 =?= fresh2 sigma s2:
-      I think so, if we have a good fresh2 function
-      *)
-      admit.
-    }
-    rewrite H_xeq.
-    rename x_s2 into x'.
+    rewrite (step_preserves_fresh sigma h).
+    remember (fresh2 sigma s2) as x'.
     apply step_abs.
-    assert (sigma [[rename x x' s1]] = ((x, tmvar x')::sigma) [[s1]]).
-    {
-      (* This is not exactly true, since rename does not create fresh vars and stuff
-        But it is "kind of true" , lol.
-
-        So I guess we have to change capms to not unnecessarily rename?
-        I would rather not ;) Maybe we can strengthen IHh to include this case.
-        Or we change rename to do fresh?
-      *)
-      admit.
-    }
-    assert (sigma [[rename x x' s2]] = ((x, tmvar x')::sigma) [[s2]]) by admit.
-    specialize (IHh ((x, tmvar x')::sigma)).
-    rewrite -> H.
-    rewrite -> H0.
+    rewrite ren_sub_compose.
+    rewrite ren_sub_compose.
     apply IHh.
-Admitted.
+Qed.
 
 (** **** Many-Step Reduction *)
 
@@ -227,6 +240,7 @@ Proof.
   elim: s sigma tau; intros; asimpl; eauto with red_congr.
 Qed. *)
 
+
 (* NOTE: A little pen and paper study strongly suggests that this is still true for named. *)
 (* NOTE: At first I would expect that it would step on the right hand side (instead of multistep=red)
     but it doesnt because of the following example:
@@ -239,22 +253,13 @@ Qed. *)
     step_beta in two different places.
     *)
 
-(* Should we add the assumption that we are always substing in fresh stuff? *)
-(* Fresh with respect to what? *)
-Fixpoint mren (rho : list (string * string)) (T : term) : term :=
-  match T with
-  | tmvar Y => match lookup Y rho with
-              | Some Z => tmvar Z
-              | None => tmvar Y
-              end
-  | tmlam Y K1 T_body => let rho' := drop Y rho in (* What if Y in rhs of rho*)
-                        tmlam Y K1 (mren rho' T_body)
-  | tmapp T1 T2 => tmapp (mren rho T1) (mren rho T2)
-end.
+(* TODO: cant we make it a relation? mren rho1 (mren rho2 s) in Mren s*)
+Lemma ren_comp rho1 rho2 s : exists rho', mren rho1 (mren rho2 s) = mren rho' s.
+Proof.
+  (* TODO: Figure out on pen and paper first.*)
+Admitted.
 
-Lemma ren_id s : mren nil s = s.
-Proof. Admitted.
-
+(* Strengthen IH for red_beta*)
 Lemma red_beta_ren x s t1 t2 rho : step t1 t2 -> red ([x := t1] (mren rho s)) ([x := t2] (mren rho s)).
 Proof.
   elim: s rho t1 t2 => [Y|Y K1 T_body IH|T1 IH1 T2 IH2] rho t1 t2 Hstep.
@@ -286,27 +291,26 @@ Proof.
         -- apply star1.
            assumption.
         -- apply starR.
-  - simpl.
+  - (* lambda abstraction *)
+    simpl.
     rewrite capms_equation_2.
     rewrite capms_equation_2.
     simpl.
     remember (fresh2 [(x, t1)] (mren (drop Y rho) T_body)) as x'.
     remember (fresh2 [(x, t2)] (mren (drop Y rho) T_body)) as x2.
-    assert (H_xeq: x' = x2). {
-      (* by reduction does not change ftv *)
-      admit.
-    }
-    rewrite <- H_xeq.
+    rewrite (step_preserves_fresh_sigma (mren (drop Y rho) T_body) x Hstep) in Heqx'.
+    rewrite <- Heqx2 in Heqx'.
+    rewrite <- Heqx'.
     remember (drop Y rho) as rho'.
     apply red_abs.
-    assert (rename Y x' (mren rho' T_body) = mren ((Y, x')::rho') T_body).
+    
+    assert (exists rho'', rename Y x' (mren rho' T_body) = mren rho'' T_body).
     {
-      (* Only true if Y not in rhs of rho'?
-      I think it shouldnt be by some freshness criterium, but even if it is, we can
-      do something else. *)
-      admit.
+      apply ren_comp.
     }
+    destruct H as [rho'' H].
     rewrite H.
+    
     apply IH.
     assumption.
   - rewrite capms_equation_3.
@@ -316,14 +320,13 @@ Proof.
       assumption.
     + apply IH2.
       assumption.
-Admitted.
+Qed.
 
 Lemma red_beta x s t1 t2 : step t1 t2 -> red ([x := t1] s) ([x := t2] s).
 Proof. 
   move=> h. 
-  (* apply red_beta_ren with empty rho*)
   apply red_beta_ren with (rho := nil) (x := x) (s := s) in h.
-  rewrite ren_id in h.
+  rewrite mren_id in h.
   assumption.
 Qed.
 
